clean up EcodeTree and HedgeParser to handle one less Hint

VerifiedFilter/Parser/HedgeParser.lean
@@ -35,7 +35,7 @@ abbrev ParseStack α := Stack (Hedge α)
 inductive CurrentState (α: Type) where
   | unknown (children: Hedge α)
   | opened (nexts: Hedge α)
-  | field (f: α) (children: Hedge α)
+  | node (node: Hedge.Node α)
   | eof
 
 structure ParserState α where
@@ -73,35 +73,12 @@ noncomputable def CurrentState.size (s: CurrentState α): Nat :=
   -- unknown needs to be the larger than opened, since it is the next state.
   | CurrentState.unknown hedge => 4 + Hedge.size hedge
   -- field needs to be larger than opened, since opened follows from field.
-  | CurrentState.field _ hedge => 3 + Hedge.size hedge
+  | CurrentState.node (Hedge.Node.node _ children) => 3 + Hedge.size children
   -- opened is always the second state, but also follows from field, so it needs to be smaller than unknown and field.
   | CurrentState.opened hedge => 2 + Hedge.size hedge
   -- eof
   | CurrentState.eof => 0
 
--- When calling next, none of the states grow the stack, except for:
--- ParserState.opened (t::nexts) and ParserState.value _ (t::nexts)
---   where t = Hedge.Node.node f children
---         children ≠ []
---         children ≠ [Hedge.Node.node v []]
--- These result in two states:
---   Stack.setCurrentM (ParserState.opened nexts)
---   Stack.pushM (ParserState.field f children)
--- We need to make sure that these two states together are smaller than the previous state.
--- This implies that we need show that the stack gets smaller as it grows in these two cases:
---   theorem sizeOf_opened_gt_push: ParserState.opened (t::nexts)  > ParserState.opened nexts + ParserState.field f children
---   theorem sizeOf_value_gt_push: ParserState.value _ (t::nexts) > ParserState.opened nexts + ParserState.field f children
--- While also making sure that as the stack shrinks for these two cases that it also gets smaller:
---   theorem sizeOf_value_gt_popped_value: x + ParserState.value _ [] > x
---   theorem sizeOf_opened_gt_popped_opened: x + ParserState.opened [] > x
--- Otherwise we also need to make sure the following equations hold:
---   theorem sizeOf_unknown_gt_opened: ParserState.unknown hedge > ParserState.opened hedge
---   theorem sizeOf_value_value_gt_value:  ParserState.value _ ((Hedge.Node.node v [])::nexts) > ParserState.value v nexts
---   theorem sizeOf_opened_value_gt_value: ParserState.opened ((Hedge.Node.node v [])::nexts) > ParserState.value v nexts
---   theorem sizeOf_value_pair_gt_pair:  ParserState.value _ ((Hedge.Node.node f [Hedge.Node.node v []])::nexts) > ParserState.pair f v nexts
---   theorem sizeOf_opened_pair_gt_pair: ParserState.opened ((Hedge.Node.node f [Hedge.Node.node v []])::nexts) > ParserState.pair f v nexts
---   theorem sizeOf_pair_gt_value: ParserState.pair _ v nexts > ParserState.value v nexts
---   theorem sizeOf_field_gt_opened: ParserState.field _ children > ParserState.opened children
 @[simp]
 noncomputable def ParserState.size (s: ParserState α): Nat :=
   s.current.size + s.stack.size
@@ -122,15 +99,6 @@ def pop
     set (σ := CurrentState α) CurrentState.eof
     return ()
 
-def nextNode
-  [Monad m] [Debug m] [MonadExcept String m] [MonadStateOf (CurrentState α) m] [MonadStateOf (ParseStack α) m]
-  (current: Hedge.Node α) (nexts: Hedge α): m Hint := do
-  match current with
-  | Hedge.Node.node f children =>
-    Stack.pushM nexts
-    set (CurrentState.field f children)
-    return Hint.value
-
 def next
   [Monad m] [Debug m] [MonadExcept String m] [MonadState (CurrentState α) m] [MonadStateOf (CurrentState α) m] [MonadStateOf (ParseStack α) m]
   : m Hint := do
@@ -143,9 +111,11 @@ def next
   | CurrentState.opened [] =>
     pop (α := α)
     return Hint.leave
-  | CurrentState.opened (t::ts) =>
-    nextNode t ts
-  | CurrentState.field _ children =>
+  | CurrentState.opened (current::nexts) =>
+    Stack.pushM nexts
+    set (CurrentState.node current)
+    return Hint.value
+  | CurrentState.node (Hedge.Node.node _ children) =>
     _ <- set (CurrentState.opened children)
     return Hint.enter
   | CurrentState.eof =>
@@ -159,7 +129,7 @@ def skip
   match curr with
   | CurrentState.unknown _ => pop (α := α)
   | CurrentState.opened _ => pop (α := α)
-  | CurrentState.field _ _ => pop (α := α)
+  | CurrentState.node _ => pop (α := α)
   | CurrentState.eof => return ()
   return ()
 
@@ -171,7 +141,7 @@ def token
   match curr with
   | CurrentState.unknown _ => throw "unknown"
   | CurrentState.opened _ => throw "unknown"
-  | CurrentState.field f _ => return f
+  | CurrentState.node (Hedge.Node.node label _) => return label
   | CurrentState.eof => throw "unknown"
 
 instance [Monad m] [Debug m] [MonadExcept String m] [MonadState (CurrentState α) m] [MonadStateOf (CurrentState α) m] [MonadStateOf (ParseStack α) m] : Parser m α where
@@ -238,7 +208,7 @@ def run (x: HedgeParser α β) (s: ParserState α): Except String (β × (Parser
 def runTree (x: HedgeParser α β) (t: Hedge.Node α): Except String β :=
   StateT.run' x (ParserState.mk' t)
 
-theorem next_unknown_gt_opened:
+theorem next_unknown_opened:
   run next (ParserState.mk (CurrentState.unknown children) stack) =
   Except.ok (Hint.enter, ParserState.mk (CurrentState.opened children) stack) := by
   simp [run, next, Debug.debug]
@@ -251,196 +221,41 @@ theorem sizeOf_unknown_gt_opened:
   sizeOf (ParserState.mk (CurrentState.opened children) stack) := by
   simp [sizeOf]
 
--- theorem next_value_value_gt_value:
---   run next (ParserState.mk (CurrentState.value v' ((Hedge.Node.node v [])::siblings)) stack) =
---   Except.ok (Hint.value, ParserState.mk (CurrentState.value v siblings) stack) := by
---   simp [run, next, nextNode, Debug.debug]
---   simp_monads
---   simp [getCurrent, setCurrent]
---   simp_monads
-
--- theorem sizeOf_value_value_gt_value:
---   sizeOf (ParserState.mk (CurrentState.value v' ((Hedge.Node.node v [])::siblings)) stack) >
---   sizeOf (ParserState.mk (CurrentState.value v siblings) stack) := by
---   simp [sizeOf]
-
--- theorem next_opened_value_gt_value:
---   run next (ParserState.mk (CurrentState.opened ((Hedge.Node.node v [])::siblings)) stack) =
---   Except.ok (Hint.value, ParserState.mk (CurrentState.value v siblings) stack) := by
---   simp [run, next, nextNode, Debug.debug]
---   simp_monads
---   simp [getCurrent, setCurrent]
---   simp_monads
-
--- theorem sizeOf_opened_value_gt_value:
---   sizeOf (ParserState.mk (CurrentState.opened ((Hedge.Node.node v [])::siblings)) stack) >
---   sizeOf (ParserState.mk (CurrentState.value v siblings) stack) := by
---   simp [sizeOf]
-
--- theorem next_value_pair_gt_pair:
---   run next (ParserState.mk (CurrentState.value v' ((Hedge.Node.node f [Hedge.Node.node v []])::siblings)) stack) =
---   Except.ok (Hint.value, ParserState.mk (CurrentState.pair f v siblings) stack) := by
---   simp [run, next, nextNode, Debug.debug]
---   simp_monads
---   simp [getCurrent, setCurrent]
---   simp_monads
-
--- theorem sizeOf_value_pair_gt_pair:
---   sizeOf (ParserState.mk (CurrentState.value v' ((Hedge.Node.node f [Hedge.Node.node v []])::siblings)) stack) >
---   sizeOf (ParserState.mk (CurrentState.pair f v siblings) stack) := by
---   simp +arith [sizeOf]
-
--- theorem next_opened_pair_gt_pair:
---   run next (ParserState.mk (CurrentState.opened ((Hedge.Node.node f [Hedge.Node.node v []])::siblings)) stack) =
---   Except.ok (Hint.value, ParserState.mk (CurrentState.pair f v siblings) stack) := by
---   simp [run, next, nextNode, Debug.debug]
---   simp_monads
---   simp [getCurrent, setCurrent]
---   simp_monads
-
--- theorem sizeOf_opened_pair_gt_pair:
---   sizeOf (ParserState.mk (CurrentState.opened ((Hedge.Node.node f [Hedge.Node.node v []])::siblings)) stack) >
---   sizeOf (ParserState.mk (CurrentState.pair f v siblings) stack) := by
---   simp +arith [sizeOf]
-
--- theorem next_pair_gt_value:
---   run next (ParserState.mk (CurrentState.pair _k v siblings) stack) =
---   Except.ok (Hint.value, ParserState.mk (CurrentState.value v siblings) stack) := by
---   simp [run, next, nextNode, Debug.debug]
---   simp_monads
---   simp [getCurrent, setCurrent]
---   simp_monads
-
--- theorem sizeOf_pair_gt_value:
---   sizeOf (ParserState.mk (CurrentState.pair _k v siblings) stack) >
---   sizeOf (ParserState.mk (CurrentState.value v siblings) stack) := by
---   simp [sizeOf]
-
-theorem next_field_gt_opened:
-  run next (ParserState.mk (CurrentState.field f' children) stack) =
+theorem next_node_opened:
+  run next (ParserState.mk (CurrentState.node (Hedge.Node.node f' children)) stack) =
   Except.ok (Hint.enter, ParserState.mk (CurrentState.opened children) stack) := by
-  simp [run, next, nextNode, Debug.debug]
+  simp [run, next, Debug.debug]
   simp_monads
   simp [getCurrent, setCurrent]
   simp_monads
 
-theorem sizeOf_field_gt_opened:
-  sizeOf (ParserState.mk (CurrentState.field f' children) stack) >
+theorem sizeOf_node_gt_opened:
+  sizeOf (ParserState.mk (CurrentState.node (Hedge.Node.node f' children)) stack) >
   sizeOf (ParserState.mk (CurrentState.opened children) stack) := by
   simp [sizeOf]
 
-theorem next_opened_gt_push
-  {fchildren: Hedge α}
-  -- if not a value and not a pair
-  (hc: (∃ v vchild vchildren, fchildren = [Hedge.Node.node v (vchild::vchildren)])
-    \/ (∃ fchild1 fchild2 fchilds, fchildren = fchild1::fchild2::fchilds)):
+theorem next_opened_push
+  {fchildren: Hedge α}:
   run next (ParserState.mk ((CurrentState.opened ((Hedge.Node.node f fchildren)::siblings))) stack) =
-  Except.ok (Hint.value, ParserState.mk (CurrentState.field f fchildren) (siblings::stack)) := by
-  cases hc with
-  | inl hc =>
-    obtain ⟨ v, vchild, vchildren, hc ⟩ := hc
-    rw [hc]
-    simp [run, next, nextNode, Debug.debug]
-    simp_monads
-    simp [getCurrent, setCurrent]
-    simp_monads
-    simp [Stack.pushM]
-    simp_monads
-    simp [getStack, setStack]
-    simp_monads
-  | inr hc =>
-    obtain ⟨ fchild1, fchild2, fchilds, hc ⟩ := hc
-    rw [hc]
-    simp [run, next, nextNode, Debug.debug]
-    simp_monads
-    simp [getCurrent, setCurrent]
-    simp_monads
-    simp [Stack.pushM]
-    simp_monads
-    simp [getStack, setStack]
-    simp_monads
+  Except.ok (Hint.value, ParserState.mk (CurrentState.node (Hedge.Node.node f fchildren)) (siblings::stack)) := by
+  simp [run, next, Debug.debug]
+  simp_monads
+  simp [getCurrent, setCurrent]
+  simp_monads
+  simp [Stack.pushM]
+  simp_monads
+  simp [getStack, setStack]
+  simp_monads
 
 theorem sizeOf_opened_gt_push:
   sizeOf (ParserState.mk ((CurrentState.opened ((Hedge.Node.node f children)::siblings))) stack) >
-  sizeOf (ParserState.mk (CurrentState.field f children) (siblings::stack)) := by
+  sizeOf (ParserState.mk (CurrentState.node (Hedge.Node.node f children)) (siblings::stack)) := by
   simp +arith [sizeOf]
 
--- run next (ParserState.mk (CurrentState.value v' ((Hedge.Node.node f [Hedge.Node.node v []])::siblings)) stack) =
--- run next (ParserState.mk (CurrentState.value v' ((Hedge.Node.node v [])::siblings)) stack) =
--- theorem next_value_gt_push
---   {fchildren: Hedge α}
---   -- if not a value and not a pair
---   (hc: (∃ v vchild vchildren, fchildren = [Hedge.Node.node v (vchild::vchildren)])
---     \/ (∃ fchild1 fchild2 fchilds, fchildren = fchild1::fchild2::fchilds)):
---   run next (ParserState.mk (CurrentState.value v ((Hedge.Node.node f fchildren)::fsiblings)) stack) =
---   Except.ok (Hint.value, ParserState.mk (CurrentState.field f fchildren) (fsiblings::stack)) := by
---   cases hc with
---   | inl hc =>
---     obtain ⟨ v, vchild, vchildren, hc ⟩ := hc
---     rw [hc]
---     simp [run, next, nextNode, Debug.debug]
---     simp_monads
---     simp [getCurrent, setCurrent]
---     simp_monads
---     simp [Stack.pushM]
---     simp_monads
---     simp [getStack, setStack]
---     simp_monads
---   | inr hc =>
---     obtain ⟨ fchild1, fchild2, fchilds, hc ⟩ := hc
---     rw [hc]
---     simp [run, next, nextNode, Debug.debug]
---     simp_monads
---     simp [getCurrent, setCurrent]
---     simp_monads
---     simp [Stack.pushM]
---     simp_monads
---     simp [getStack, setStack]
---     simp_monads
-
--- theorem sizeOf_value_gt_push:
---   sizeOf (ParserState.mk ((CurrentState.value v ((Hedge.Node.node f children)::siblings))) stack) >
---   sizeOf (ParserState.mk (CurrentState.field f children) (siblings::stack)) := by
---   simp +arith [sizeOf]
-
--- theorem next_value_gt_popped_value_eof {α: Type} (v: α):
---   run next (ParserState.mk (α := α) (CurrentState.value v []) []) =
---   Except.ok (Hint.leave, ParserState.mk (α := α) CurrentState.eof []) := by
---   simp [run, next, nextNode, Debug.debug]
---   simp_monads
---   simp [getCurrent, setCurrent]
---   simp_monads
---   simp [pop, Stack.popM?]
---   simp_monads
---   simp [getStack, setCurrent]
---   simp_monads
-
--- theorem sizeOf_value_gt_popped_value_eof {α: Type}:
---   sizeOf (ParserState.mk (CurrentState.value _v []) []) >
---   sizeOf (ParserState.mk (α := α) CurrentState.eof []) := by
---   simp [sizeOf]
-
--- theorem next_value_gt_popped_value_more:
---   run next (ParserState.mk (CurrentState.value _v []) (elem::stack)) =
---   Except.ok (Hint.leave, ParserState.mk (CurrentState.opened elem) stack) := by
---   simp [run, next, nextNode, Debug.debug]
---   simp_monads
---   simp [getCurrent, setCurrent]
---   simp_monads
---   simp [pop, Stack.popM?]
---   simp_monads
---   simp [getStack, setStack, setCurrent]
---   simp_monads
-
--- theorem sizeOf_value_gt_popped_value_more:
---   sizeOf (ParserState.mk (CurrentState.value _v []) (elem::stack)) >
---   sizeOf (ParserState.mk (CurrentState.opened elem) stack) := by
---   simp +arith [sizeOf]
-
-theorem next_opened_gt_popped_opened_eof {α: Type}:
+theorem next_opened_popped_opened_eof {α: Type}:
   run next (ParserState.mk (α := α) (CurrentState.opened []) []) =
   Except.ok (Hint.leave, ParserState.mk (α := α) CurrentState.eof []) := by
-  simp [run, next, nextNode, Debug.debug]
+  simp [run, next, Debug.debug]
   simp_monads
   simp [getCurrent, setCurrent]
   simp_monads
@@ -454,10 +269,10 @@ theorem sizeOf_opened_gt_popped_opened_eof {α: Type}:
   sizeOf (ParserState.mk (α := α) CurrentState.eof []) := by
   simp [sizeOf]
 
-theorem next_opened_gt_popped_opened_more:
+theorem next_opened_popped_opened_more:
   run next (ParserState.mk (CurrentState.opened []) (elem::stack)) =
   Except.ok (Hint.leave, ParserState.mk (CurrentState.opened elem) stack) := by
-  simp [run, next, nextNode, Debug.debug]
+  simp [run, next, Debug.debug]
   simp_monads
   simp [getCurrent, setCurrent]
   simp_monads
@@ -492,10 +307,10 @@ open TokenHedge (strnode)
   (strnode "a" [])
   = Except.ok ["{", "V", "{", "}", "}"]
 
--- #guard runTree
---   (walk [Action.next, Action.next, Action.next, Action.next, Action.next, Action.next, Action.next, Action.next])
---   (strnode "a" [strnode "b" [], strnode "c" [strnode "d" []]]) =
---   Except.ok ["{", "V", "{", "V", "V", "V", "}", "}"]
+#guard runTree
+  (walk [Action.next, Action.next, Action.next, Action.next, Action.next, Action.next, Action.next, Action.next, Action.next, Action.next, Action.next, Action.next, Action.next, Action.next])
+  (strnode "a" [strnode "b" [], strnode "c" [strnode "d" []]])
+  = Except.ok ["{", "V", "{", "V", "{", "}", "V", "{", "V", "{", "}", "}", "}", "}"]
 
 -- walk next just two
 #guard runTree
@@ -504,22 +319,36 @@ open TokenHedge (strnode)
   = Except.ok ["{", "V"]
 
 -- walk next to end
--- #guard runTree
---   (walk [Action.next, Action.next, Action.next, Action.next, Action.next, Action.next, Action.next, Action.next, Action.next])
---   (strnode "a" [strnode "b" [], strnode "c" [strnode "d" []]])
---   = Except.ok ["{", "V", "{", "V", "V", "V", "}", "}", "$"]
+#guard runTree
+  (walk [Action.next, Action.next, Action.next, Action.next, Action.next, Action.next, Action.next, Action.next, Action.next, Action.next, Action.next, Action.next, Action.next, Action.next, Action.next])
+  (strnode "a" [strnode "b" [], strnode "c" [strnode "d" []]])
+  = Except.ok ["{", "V", "{", "V", "{", "}", "V", "{", "V", "{", "}", "}", "}", "}", "$"]
 
 -- walk next to end and tokenize all
--- #guard runTree
---   (walk [Action.next, Action.next, Action.token, Action.next, Action.next, Action.token, Action.next, Action.token, Action.next, Action.token, Action.next, Action.next, Action.next])
---   (strnode "a" [strnode "b" [], strnode "c" [strnode "d" []]])
---   = Except.ok ["{", "V", "a", "{", "V", "b", "V", "c", "V", "d", "}", "}", "$"]
-
--- walk next to end and tokenize all
--- #guard runTree
---   (walk [Action.next, Action.next, Action.token, Action.next, Action.next, Action.token, Action.next, Action.token, Action.next, Action.token, Action.next, Action.next, Action.next])
---   (strnode "a" [strnode "b" [], strnode "c" [strnode "d" []]])
---   = Except.ok ["{", "V", "a", "{", "V", "b", "V", "c", "V", "d", "}", "}", "$"]
+#guard runTree
+  (walk [
+    Action.next,
+    Action.next,
+    Action.token,
+    Action.next,
+    Action.next,
+    Action.token,
+    Action.next,
+    Action.next,
+    Action.next,
+    Action.token,
+    Action.next,
+    Action.next,
+    Action.token,
+    Action.next,
+    Action.next,
+    Action.next,
+    Action.next,
+    Action.next,
+    Action.next,
+  ])
+  (strnode "a" [strnode "b" [], strnode "c" [strnode "d" []]])
+  = Except.ok ["{", "V", "a", "{", "V", "b", "{", "}", "V", "c", "{", "V", "d", "{", "}", "}", "}", "}", "$"]
 
 -- walk skip
 #guard runTree
@@ -551,177 +380,72 @@ open TokenHedge (strnode)
   (strnode "a" [strnode "b" [], strnode "c" [strnode "d" []]]) =
   Except.ok ["{", "V", "a", "{", "}", "$"]
 
--- walk next next token next next token skip
--- #guard runTree
---   (walk [Action.next, Action.next, Action.token, Action.next, Action.next, Action.token, Action.skip, Action.next, Action.next])
---   (strnode "a" [strnode "b" [], strnode "c" [strnode "d" []]]) =
---   Except.ok ["{", "V", "a", "{", "V", "b", "}", "$"]
+-- walk skip rest of fields after b
+#guard runTree
+  (walk [
+      Action.next, Action.next, Action.token,
+      Action.next, Action.next, Action.token,
+      Action.next, Action.next,
+      Action.skip,
+      Action.next,
+      Action.next])
+  (strnode "a" [strnode "b" [], strnode "c" [strnode "d" []]])
+  = Except.ok ["{", "V", "a", "{", "V", "b", "{", "}", "}", "$"]
 
--- walk next next token next next token next token skip
--- #guard runTree
---   (walk [Action.next, Action.next, Action.token, Action.next, Action.next, Action.token, Action.next, Action.token, Action.skip, Action.next, Action.next, Action.next])
---   (strnode "a" [strnode "b" [], strnode "c" [strnode "d" []]]) =
---   Except.ok ["{", "V", "a", "{", "V", "b", "V", "c", "}", "}", "$"]
+-- walk skip c's children
+#guard runTree
+  (walk [Action.next, Action.next, Action.token, Action.next, Action.next, Action.token, Action.next, Action.next, Action.next, Action.token, Action.skip, Action.next, Action.next, Action.next])
+  (strnode "a" [strnode "b" [], strnode "c" [strnode "d" []]])
+  = Except.ok ["{", "V", "a", "{", "V", "b", "{", "}", "V", "c", "}", "}", "$"]
 
--- theorem next_decreases_size_of_parserstate
---   {hint: Hint}
---   {thisParserState nextParserState: ParserState α}
---   (hneof: hint ≠ Hint.eof)
---   (h: Except.ok (hint, nextParserState) = run next thisParserState):
---   sizeOf nextParserState < sizeOf thisParserState := by
---   have h' := Eq.symm h
---   clear h
---   have h := congrArg (Except.map (fun x => x.snd)) h'
---   simp [Except.map] at h
---   cases thisParserState with
---   | mk thisCurrent thisStack =>
---   cases thisCurrent with
---   | unknown xs =>
---     rw [next_unknown_gt_opened] at h
---     simp at h
---     rw [<- h]
---     exact sizeOf_unknown_gt_opened
---   | opened xs =>
---     cases xs with
---     | nil =>
---       cases thisStack with
---       | nil =>
---         rw [next_opened_gt_popped_opened_eof] at h
---         simp at h
---         rw [<- h]
---         exact sizeOf_opened_gt_popped_opened_eof
---       | cons s' ss' =>
---         rw [next_opened_gt_popped_opened_more] at h
---         simp at h
---         rw [<- h]
---         exact sizeOf_opened_gt_popped_opened_more
---     | cons tree fsiblings =>
---       cases tree with
---       | node f v =>
---         cases v with
---         | nil =>
---           -- is value
---           rw [next_opened_value_gt_value] at h
---           simp at h
---           rw [<- h]
---           exact sizeOf_opened_value_gt_value
---         | cons v vsiblings =>
---           -- is pair or field
---           cases v with
---           | node v vchildren =>
---             cases vchildren with
---             | nil =>
---               cases vsiblings with
---               | nil =>
---                 -- is pair
---                 rw [next_opened_pair_gt_pair] at h
---                 simp at h
---                 rw [<- h]
---                 exact sizeOf_opened_pair_gt_pair
---               | cons vsibling vsiblings =>
---                 -- is field
---                 rw [next_opened_gt_push] at h
---                 simp at h
---                 rw [<- h]
---                 apply sizeOf_opened_gt_push
---                 right
---                 exists Hedge.Node.node v []
---                 exists vsibling
---                 exists vsiblings
---             | cons vchild vchildren =>
---               -- if field
---               rw [next_opened_gt_push] at h
---               simp at h
---               rw [<- h]
---               apply sizeOf_opened_gt_push
---               cases vsiblings with
---               | nil =>
---                 left
---                 exists v
---                 exists vchild
---                 exists vchildren
---               | cons vsibling vsiblings =>
---                 right
---                 exists Hedge.Node.node v (vchild :: vchildren)
---                 exists vsibling
---                 exists vsiblings
---   | value x xs =>
---     cases xs with
---     | nil =>
---       cases thisStack with
---       | nil =>
---         rw [next_value_gt_popped_value_eof] at h
---         simp at h
---         rw [<- h]
---         exact sizeOf_value_gt_popped_value_eof
---       | cons s' ss' =>
---         rw [next_value_gt_popped_value_more] at h
---         simp at h
---         rw [<- h]
---         exact sizeOf_value_gt_popped_value_more
---     | cons tree fsiblings =>
---       cases tree with
---       | node f v =>
---         cases v with
---         | nil =>
---           -- is value
---           rw [next_value_value_gt_value] at h
---           simp at h
---           rw [<- h]
---           exact sizeOf_opened_value_gt_value
---         | cons v vsiblings =>
---           -- is pair or field
---           cases v with
---           | node v vchildren =>
---             cases vchildren with
---             | nil =>
---               cases vsiblings with
---               | nil =>
---                 -- is pair
---                 rw [next_value_pair_gt_pair] at h
---                 simp at h
---                 rw [<- h]
---                 exact sizeOf_opened_pair_gt_pair
---               | cons vsibling vsiblings =>
---                 -- is field
---                 rw [next_value_gt_push] at h
---                 simp at h
---                 rw [<- h]
---                 apply sizeOf_opened_gt_push
---                 right
---                 exists Hedge.Node.node v []
---                 exists vsibling
---                 exists vsiblings
---             | cons vchild vchildren =>
---               -- if field
---               rw [next_value_gt_push] at h
---               simp at h
---               rw [<- h]
---               apply sizeOf_opened_gt_push
---               cases vsiblings with
---               | nil =>
---                 left
---                 exists v
---                 exists vchild
---                 exists vchildren
---               | cons vsibling vsiblings =>
---                 right
---                 exists Hedge.Node.node v (vchild :: vchildren)
---                 exists vsibling
---                 exists vsiblings
---   | pair f v xs =>
---     rw [next_pair_gt_value] at h
---     simp at h
---     rw [<- h]
---     exact sizeOf_pair_gt_value
---   | field f xs =>
---     rw [next_field_gt_opened] at h
---     simp at h
---     rw [<- h]
---     exact sizeOf_field_gt_opened
---   | eof =>
---     rw [next_eof_gt_eof] at h'
---     simp at h'
---     obtain ⟨heof, _⟩ := h'
---     rw [<- heof] at hneof
---     contradiction
+theorem next_decreases_size_of_parserstate
+  {hint: Hint}
+  {thisParserState nextParserState: ParserState α}
+  (hneof: hint ≠ Hint.eof)
+  (h: Except.ok (hint, nextParserState) = run next thisParserState):
+  sizeOf nextParserState < sizeOf thisParserState := by
+  have h' := Eq.symm h
+  clear h
+  have h := congrArg (Except.map (fun x => x.snd)) h'
+  simp [Except.map] at h
+  cases thisParserState with
+  | mk thisCurrent thisStack =>
+  cases thisCurrent with
+  | unknown xs =>
+    rw [next_unknown_opened] at h
+    simp at h
+    rw [<- h]
+    exact sizeOf_unknown_gt_opened
+  | opened xs =>
+    cases xs with
+    | nil =>
+      cases thisStack with
+      | nil =>
+        rw [next_opened_popped_opened_eof] at h
+        simp at h
+        rw [<- h]
+        exact sizeOf_opened_gt_popped_opened_eof
+      | cons s' ss' =>
+        rw [next_opened_popped_opened_more] at h
+        simp at h
+        rw [<- h]
+        exact sizeOf_opened_gt_popped_opened_more
+    | cons tree fsiblings =>
+      cases tree with
+      | node f v =>
+        rw [next_opened_push] at h
+        simp at h
+        rw [<- h]
+        exact sizeOf_opened_gt_push
+  | node n =>
+    cases n
+    rw [next_node_opened] at h
+    simp at h
+    rw [<- h]
+    exact sizeOf_node_gt_opened
+  | eof =>
+    rw [next_eof_gt_eof] at h'
+    simp at h'
+    obtain ⟨heof, _⟩ := h'
+    rw [<- heof] at hneof
+    contradiction
